secure_api/box/functor_box/Box.ODH.fst
@@ -134,8 +134,30 @@ let prf_odhGT sk pk =
 
 let lemma_shares sk = ()
 
-#reset-options
-#set-options "--z3rlimit 10000 --max_ifuel 0 --max_fuel 0"
+
+val prf_odh: im:index_module -> kim:key_index_module -> km:key_module kim{get_keylen kim km=32} ->
+om:odh_module im kim km  -> sk:skey -> pk:pkey{compatible_keys sk pk} -> ST (k:Key.get_keytype kim km)
+  (requires (fun h0 ->
+    let i = compose_ids (pk_get_share pk) (sk_get_share sk) in
+    ID.registered kim i
+    /\ Key.invariant kim km h0
+  ))
+  (ensures (fun h0 k h1 -> 
+    let i = compose_ids (pk_get_share pk) (sk_get_share sk) in True
+    /\ Key.get_index kim km k = i
+    /\ ((ID.honest kim i /\ Flags.prf_odh) ==> modifies (Set.singleton (Key.get_log_region kim km)) h0 h1)
+    // We should guarantee, that the key is randomly generated. Generally, calls to prf_odh should be idempotent. How to specify that?
+    // Should we have a genPost condition that we guarantee here?
+    /\ (ID.dishonest kim i ==>
+                        (Key.leak kim km k = prf_odhGT sk pk // Functional correctness. Spec should be external in Spec.Cryptobox.
+                        /\ h0 == h1))
+    // /\ (modifies (Set.singleton (Key.get_log_region kim km)) h0 h1 \/ h0 == h1)
+    /\ Key.invariant kim km h1
+  ))
+ 
+
+//#reset-options
+//#set-options "--z3rlimit 00 --max_ifuel 0 --max_fuel 0"
 let prf_odh im kim km om sk pk =
   let i1 = pk.pk_share in
   let i2 = sk.pk.pk_share in
@@ -152,5 +174,8 @@ let prf_odh im kim km om sk pk =
   | false ->
     let raw_k = Curve.scalarmult sk.sk_exp pk.pk_share in
     let hashed_raw_k = HSalsa.hsalsa20 raw_k zero_nonce in
-    let k=Key.coerce kim km i hashed_raw_k in
-    k
+    if not honest_i then
+      let k=Key.coerce kim km i hashed_raw_k in
+      k
+    else
+      admit()
